Weidenbach_Book/Watched_Literals/Watched_Literals_Watch_List_Simp.thy
@@ -9,9 +9,9 @@ no_notation funcset (infixr "\<rightarrow>" 60)
 definition cdcl_twl_full_restart_wl_GC_prog where
   \<open>cdcl_twl_full_restart_wl_GC_prog S = do {
   ASSERT(cdcl_twl_full_restart_wl_GC_prog_pre S);
-  \<comment> \<open>\<^text>\<open>S' \<leftarrow> cdcl_twl_local_restart_wl_spec0 S;\<close>\<close>
+  S' \<leftarrow> cdcl_twl_local_restart_wl_spec0 S;
   \<comment> \<open>\<^text>\<open>S' \<leftarrow> simplify_clauses_with_unit_st_wl S';\<close>\<close>
-  T \<leftarrow> remove_one_annot_true_clause_imp_wl S;
+  T \<leftarrow> remove_one_annot_true_clause_imp_wl S';
   ASSERT(mark_to_delete_clauses_wl_pre T);
   U \<leftarrow> mark_to_delete_clauses_wl2 T;
   V \<leftarrow> cdcl_GC_clauses_wl U;
@@ -43,6 +43,52 @@ lemma cdcl_twl_full_restart_wl_GC_prog:
     by (rule cdcl_twl_full_restart_wl_GC_prog_post_correct_watching)
   done
 
+definition cdcl_twl_full_restart_inprocess_wl_prog where
+  \<open>cdcl_twl_full_restart_inprocess_wl_prog S = do {
+  ASSERT(cdcl_twl_full_restart_wl_GC_prog_pre S);
+  S' \<leftarrow> cdcl_twl_local_restart_wl_spec0 S;
+  S' \<leftarrow> simplify_clauses_with_unit_st_wl S';
+  if get_conflict_wl S' \<noteq> None
+  then RETURN S'
+  else do {
+    T \<leftarrow> remove_one_annot_true_clause_imp_wl S';
+    ASSERT(mark_to_delete_clauses_wl_pre T);
+    U \<leftarrow> mark_to_delete_clauses_wl2 T;
+    V \<leftarrow> cdcl_GC_clauses_wl U;
+    ASSERT(cdcl_twl_full_restart_wl_GC_prog_post S V);
+    RETURN V
+  }
+  }\<close>
+
+    find_theorems simplify_clauses_with_unit_st_wl simplify_clauses_with_unit_st
+lemma cdcl_twl_full_restart_wl_GC_prog:
+  \<open>(cdcl_twl_full_restart_inprocess_wl_prog, cdcl_twl_full_restart_inprocess_l) \<in>
+    {(S::'v twl_st_wl, S').
+       (S, S') \<in> state_wl_l None \<and> correct_watching' S \<and> literals_are_\<L>\<^sub>i\<^sub>n' S} \<rightarrow>\<^sub>f
+     \<langle>{(S::'v twl_st_wl, S').
+       (S, S') \<in> state_wl_l None \<and> correct_watching S \<and> blits_in_\<L>\<^sub>i\<^sub>n S}\<rangle>nres_rel\<close>
+  unfolding cdcl_twl_full_restart_inprocess_wl_prog_def cdcl_twl_full_restart_inprocess_l_def
+  apply (intro frefI nres_relI)
+  apply (refine_vcg
+    remove_one_annot_true_clause_imp_wl_remove_one_annot_true_clause_imp[THEN fref_to_Down]
+    mark_to_delete_clauses_wl_mark_to_delete_clauses_l2[THEN fref_to_Down]
+    cdcl_GC_clauses_wl_cdcl_GC_clauses[THEN fref_to_Down]
+    cdcl_twl_local_restart_wl_spec0_cdcl_twl_local_restart_l_spec0
+    simplify_clauses_with_unit_st_wl_simplify_clause_with_unit_st)
+  subgoal unfolding cdcl_twl_full_restart_wl_GC_prog_pre_def by blast
+  subgoal by (auto dest: correct_watching'_correct_watching'')
+    oops
+  subgoal unfolding mark_to_delete_clauses_wl_pre_def by fast
+  subgoal for x y S S' T Ta U Ua V Va
+    using cdcl_twl_full_restart_wl_GC_prog_post_correct_watching[of y Va V]
+    unfolding cdcl_twl_full_restart_wl_GC_prog_post_def
+    by fast
+  subgoal for x y S' S'a T Ta U Ua V Va
+    by (rule cdcl_twl_full_restart_wl_GC_prog_post_correct_watching)
+  done
+  
+  term cdcl_twl_full_restart_inprocess_l
+    term cdcl_twl_full_restart_l_GC_prog_pre
 
 context twl_restart_ops
 begin
